expression_eval_smallstep.v
@@ -9,17 +9,17 @@ Context `{EnvSpec K}.
 Implicit Types e : expr K.
 Implicit Types a : addr K.
 Implicit Types v : val K.
-Implicit Types av : lrval K.
+Implicit Types ν : lrval K.
 Implicit Types E : ectx K.
 
-Lemma expr_eval_ehstep Γ fs ρ e1 m av :
-  ⟦ e1 ⟧ Γ fs ρ m = Some av → is_redex e1 →
-  (**i 1). *) (∃ e2, Γ\ ρ ⊢ₕ e1, m ⇒ e2, m ∧ ⟦ e2 ⟧ Γ fs ρ m = Some av) ∨
+Lemma expr_eval_ehstep Γ fs ρ e1 m ν :
+  ⟦ e1 ⟧ Γ fs ρ m = Some ν → is_redex e1 →
+  (**i 1). *) (∃ e2, Γ\ ρ ⊢ₕ e1, m ⇒ e2, m ∧ ⟦ e2 ⟧ Γ fs ρ m = Some ν) ∨
   (**i 2). *) (∃ Ω f τs τ F Ωs vs v,
-    e1 = (call #{Ω} (ptrV (FunPtr f τs τ)) @ #{Ωs}* vs)%E ∧ av = inr v ∧
+    e1 = (call #{Ω} (ptrV (FunPtr f τs τ)) @ #{Ωs}* vs)%E ∧ ν = inr v ∧
     length Ωs = length vs ∧ fs !! f = Some F ∧ F vs = Some v).
 Proof.
-  revert e1 av. assert (∀ a v,
+  revert e1 ν. assert (∀ a v,
     mem_forced Γ a m → m !!{Γ} a = Some v → Γ\ ρ ⊢ₕ load (%a), m ⇒ #v, m).
   { intros a v Hm ?. rewrite <-Hm at 2. do_ehstep. }
   assert (∀ es vs,
@@ -39,30 +39,29 @@ Proof.
   right; eexists _,_,_,_,_,_,_,_; split_ands; eauto.
   rewrite fmap_length; eauto using Forall2_length.
 Qed.
-Lemma expr_eval_subst_ehstep Γ fs ρ m E e1 av :
-  ⟦ subst E e1 ⟧ Γ fs ρ m = Some av → is_redex e1 →
+Lemma expr_eval_subst_ehstep Γ fs ρ m E e1 ν :
+  ⟦ subst E e1 ⟧ Γ fs ρ m = Some ν → is_redex e1 →
   (**i 1). *) (∃ e2,
-    Γ\ ρ ⊢ₕ e1, m ⇒ e2, m ∧ ⟦ subst E e2 ⟧ Γ fs ρ m = Some av) ∨
+    Γ\ ρ ⊢ₕ e1, m ⇒ e2, m ∧ ⟦ subst E e2 ⟧ Γ fs ρ m = Some ν) ∨
   (**i 2). *) (∃ Ω f τs τ F Ωs vs v,
     e1 = (call #{Ω} (ptrV (FunPtr f τs τ)) @ #{Ωs}* vs)%E ∧
     length Ωs = length vs ∧ fs !! f = Some F ∧ F vs = Some v ∧
-    ⟦ subst E (# v)%E ⟧ Γ fs ρ m = Some av).
+    ⟦ subst E (# v)%E ⟧ Γ fs ρ m = Some ν).
 Proof.
-  rewrite expr_eval_subst; intros (av'&Heval'&<-) ?.
+  rewrite expr_eval_subst; intros (ν'&Heval'&<-) ?.
   destruct (expr_eval_ehstep _ _ _ _ _ _ Heval')
     as [(e2&?&?)|(Ω&f&τs&τ&F&Ωs&vs&v&->&->&?&?&?)]; trivial.
-  * left; exists e2; split; auto. apply subst_preserves_expr_eval.
-    by rewrite expr_eval_lrval.
+  * left; exists e2; split; auto using subst_preserves_expr_eval.
   * right; eexists Ω, f, τs, τ, F, Ωs, vs, v; eauto.
 Qed.
-Lemma expr_eval_sound Γ δ m k e av :
-  ⟦ e ⟧ Γ ∅ (get_stack k) m = Some av →
-  Γ\ δ ⊢ₛ State k (Expr e) m ⇒{k}* State k (Expr (%# av)) m.
+Lemma expr_eval_sound Γ δ m k e ν :
+  ⟦ e ⟧ Γ ∅ (get_stack k) m = Some ν →
+  Γ\ δ ⊢ₛ State k (Expr e) m ⇒{k}* State k (Expr (%# ν)) m.
 Proof.
   induction e as [e IH] using expr_wf_ind; intros He.
   destruct (is_nf_or_redex e) as [He'|(E&e1&?&->)].
   { by destruct He'; simplify_option_equality. }
-  destruct (expr_eval_subst_ehstep Γ ∅ (get_stack k) m E e1 av)
+  destruct (expr_eval_subst_ehstep Γ ∅ (get_stack k) m E e1 ν)
     as [(e2&?&?)|(?&?&?&?&?&?&?&?&?&?&?&?&?)]; simplify_map_equality; auto.
   econstructor; [do_cstep|]. apply IH; auto.
   rewrite !ectx_subst_size, <-Nat.add_lt_mono_l; eauto using ehstep_size.
@@ -77,12 +76,12 @@ Proof.
     | _ => progress simplify_option_equality
     end || solve_elem_of.
 Qed.
-Lemma expr_eval_complete Γ δ m1 m2 k e av :
-  Γ\ δ ⊢ₛ State k (Expr e) m1 ⇒{k}* State k (Expr (%# av)) m2 →
-  is_pure e → ⟦ e ⟧ Γ ∅ (get_stack k) m1 = Some av ∧ m1 = m2.
+Lemma expr_eval_complete Γ δ m1 m2 k e ν :
+  Γ\ δ ⊢ₛ State k (Expr e) m1 ⇒{k}* State k (Expr (%# ν)) m2 →
+  is_pure e → ⟦ e ⟧ Γ ∅ (get_stack k) m1 = Some ν ∧ m1 = m2.
 Proof.
   remember (State k (Expr e) m1) as S eqn:He; intros p; revert S p m1 e He.
-  refine (rtc_ind_l _ _ _ _); [naive_solver eauto using expr_eval_lrval|].
+  refine (rtc_ind_l _ _ _ _); [naive_solver|].
   intros S1 S2 [p Hk] p' IH m1 e -> Hsafe. revert p' Hk Hsafe IH. pattern S2.
   apply (cstep_focus_inv _ _ _ _ _ p); try (intros; solve_suffix_of); clear p.
   * intros E e1 e2 m1' -> p' p _ Hpure IH.
@@ -95,16 +94,16 @@ Proof.
     apply ectx_is_pure in Hsafe; inversion Hsafe.
   * intros E e1 -> ?? p'. inv_csteps p'; inv_cstep.
 Qed.
-Lemma expr_eval_subst_ehsafe Γ fs ρ m E e av :
-  ⟦ subst E e ⟧ Γ fs ρ m = Some av → is_redex e → Γ\ ρ ⊢ₕ safe e, m.
+Lemma expr_eval_subst_ehsafe Γ fs ρ m E e ν :
+  ⟦ subst E e ⟧ Γ fs ρ m = Some ν → is_redex e → Γ\ ρ ⊢ₕ safe e, m.
 Proof.
-  intros Heval ?. destruct (expr_eval_subst_ehstep Γ fs ρ m E e av)
+  intros Heval ?. destruct (expr_eval_subst_ehstep Γ fs ρ m E e ν)
     as [(e2&?&?)|(Ω&f&τs&τ&F&Ωs&vs&v&->&?&?&?&?)]; trivial.
   * eauto using ehsafe_step.
   * by constructor.
 Qed.
-Lemma expr_eval_cred Γ fs δ e k m av :
-  ⟦ e ⟧ Γ fs (get_stack k) m = Some av → ¬is_nf e →
+Lemma expr_eval_cred Γ fs δ e k m ν :
+  ⟦ e ⟧ Γ fs (get_stack k) m = Some ν → ¬is_nf e →
   red (cstep_in_ctx Γ δ k) (State k (Expr e) m).
 Proof.
   intros Heval He. destruct (is_nf_is_redex _ He) as (E'&e'&?&->).
